hax-lib/proof-libs/fstar/core/Core_models.Ops.Function.fst
@@ -10,13 +10,26 @@ class t_FnOnce (v_Self: Type0) (v_Args: Type0) = {
     -> Prims.Pure f_Output (f_call_once_pre x0 x1) (fun result -> f_call_once_post x0 x1 result)
 }
 
-unfold instance fnonce_arrow t u
-  : t_FnOnce (t -> u) t = {
-    f_Output = u;
-    f_call_once_pre = (fun _ _ -> true);
-    f_call_once_post = (fun (x0: t -> u) (x1: t) (res: u) -> res == x0 x1);
-    f_call_once = (fun (x0: t -> u) (x1: t) -> x0 x1);
-  } 
+class t_Fn (v_Self: Type0) (v_Args: Type0) = {
+  [@@@ FStar.Tactics.Typeclasses.no_method]_super_i0:t_FnOnce v_Self v_Args;
+  f_call_pre:self_: v_Self -> args: v_Args -> pred: Type0{true ==> pred};
+  f_call_post:v_Self -> v_Args -> (_super_i0).f_Output -> Type0;
+  f_call:x0: v_Self -> x1: v_Args
+    -> Prims.Pure (_super_i0).f_Output (f_call_pre x0 x1) (fun result -> f_call_post x0 x1 result)
+}
+
+[@@ FStar.Tactics.Typeclasses.tcinstance]
+let _ = fun (v_Self:Type0) (v_Args:Type0) {|i: t_Fn v_Self v_Args|} -> i._super_i0
+
+[@@ FStar.Tactics.Typeclasses.tcinstance]
+let impl (#v_Args #v_Out: Type0) : t_FnOnce (v_Args -> v_Out) v_Args =
+  {
+    f_Output = v_Out;
+    f_call_once_pre = (fun (self: (v_Args -> v_Out)) (args: v_Args) -> true);
+    f_call_once_post = (fun (self: (v_Args -> v_Out)) (args: v_Args) (out: v_Out) -> true);
+    f_call_once = fun (self: (v_Args -> v_Out)) (args: v_Args) -> self args
+  }
+
 unfold instance fnonce_arrow_binder t u
   : t_FnOnce (_:t -> u) t = {
     f_Output = u;
@@ -24,16 +37,3 @@ unfold instance fnonce_arrow_binder t u
     f_call_once_post = (fun (x0: (_:t -> u)) (x1: t) (res: u) -> res == x0 x1);
     f_call_once = (fun (x0: (_:t -> u)) (x1: t) -> x0 x1);
   }
-
-class t_Fn (v_Self: Type0) (v_Args: Type0) = {
-  [@@@ FStar.Tactics.Typeclasses.no_method]_super_17771448556265749037:t_FnOnce v_Self v_Args;
-  f_call_pre:self_: v_Self -> args: v_Args -> pred: Type0{true ==> pred};
-  f_call_post:v_Self -> v_Args -> (_super_17771448556265749037).f_Output -> Type0;
-  f_call:x0: v_Self -> x1: v_Args
-    -> Prims.Pure (_super_17771448556265749037).f_Output
-        (f_call_pre x0 x1)
-        (fun result -> f_call_post x0 x1 result)
-}
-
-[@@ FStar.Tactics.Typeclasses.tcinstance]
-let _ = fun (v_Self:Type0) (v_Args:Type0) {|i: t_Fn v_Self v_Args|} -> i._super_17771448556265749037
