hax-lib/proof-libs/fstar/rust_primitives/Rust_primitives.Arithmetic.fsti
@@ -1,0 +1,208 @@
+module Rust_primitives.Arithmetic
+
+open FStar.Mul
+open Rust_primitives.Integers
+
+let wrapping_add_u8 : u8 -> u8 -> u8 = add_mod
+let saturating_add_u8 : u8 -> u8 -> u8 = add_sat
+val overflowing_add_u8 : u8 -> u8 -> u8 & bool
+let wrapping_sub_u8 : u8 -> u8 -> u8 = sub_mod
+let saturating_sub_u8 : u8 -> u8 -> u8 = sub_sat
+let overflowing_sub_u8 (x y: u8): u8 & bool
+  = let sub = v x - v y in
+    let borrow = sub < 0 in
+    let out = if borrow then pow2 8 + sub else sub in
+    (mk_u8 out, borrow)
+let wrapping_mul_u8 : u8 -> u8 -> u8 = mul_mod
+val saturating_mul_u8 : u8 -> u8 -> u8
+let overflowing_mul_u8 : u8 -> u8 -> u8 & bool = mul_overflow
+let rem_euclid_u8 (x: u8) (y: u8 {v y <> 0}): u8 = x %! y
+val pow_u8 : u8 -> u32 -> u8
+val count_ones_u8 : u8 -> r:u32{v r <= 8}
+
+let wrapping_add_u16 : u16 -> u16 -> u16 = add_mod
+let saturating_add_u16 : u16 -> u16 -> u16 = add_sat
+val overflowing_add_u16 : u16 -> u16 -> u16 & bool
+let wrapping_sub_u16 : u16 -> u16 -> u16 = sub_mod
+let saturating_sub_u16 : u16 -> u16 -> u16 = sub_sat
+let overflowing_sub_u16 (x y: u16): u16 & bool
+  = let sub = v x - v y in
+    let borrow = sub < 0 in
+    let out = if borrow then pow2 16 + sub else sub in
+    (mk_u16 out, borrow)
+let wrapping_mul_u16 : u16 -> u16 -> u16 = mul_mod
+val saturating_mul_u16 : u16 -> u16 -> u16
+let overflowing_mul_u16 : u16 -> u16 -> u16 & bool = mul_overflow
+let rem_euclid_u16 (x: u16) (y: u16 {v y <> 0}): u16 = x %! y
+val pow_u16 : u16 -> u32 -> u16
+val count_ones_u16 : u16 -> r:u32{v r <= 16}
+
+let wrapping_add_u32 : u32 -> u32 -> u32 = add_mod
+let saturating_add_u32 : u32 -> u32 -> u32 = add_sat
+val overflowing_add_u32 : u32 -> u32 -> u32 & bool
+let wrapping_sub_u32 : u32 -> u32 -> u32 = sub_mod
+let saturating_sub_u32 : u32 -> u32 -> u32 = sub_sat
+let overflowing_sub_u32 (x y: u32): u32 & bool
+  = let sub = v x - v y in
+    let borrow = sub < 0 in
+    let out = if borrow then pow2 32 + sub else sub in
+    (mk_u32 out, borrow)
+let wrapping_mul_u32 : u32 -> u32 -> u32 = mul_mod
+val saturating_mul_u32 : u32 -> u32 -> u32
+let overflowing_mul_u32 : u32 -> u32 -> u32 & bool = mul_overflow
+let rem_euclid_u32 (x: u32) (y: u32 {v y <> 0}): u32 = x %! y
+val pow_u32 : u32 -> u32 -> u32
+val count_ones_u32 : u32 -> r:u32{v r <= 32}
+
+let wrapping_add_u64 : u64 -> u64 -> u64 = add_mod
+let saturating_add_u64 : u64 -> u64 -> u64 = add_sat
+val overflowing_add_u64 : u64 -> u64 -> u64 & bool
+let wrapping_sub_u64 : u64 -> u64 -> u64 = sub_mod
+let saturating_sub_u64 : u64 -> u64 -> u64 = sub_sat
+let overflowing_sub_u64 (x y: u64): u64 & bool
+  = let sub = v x - v y in
+    let borrow = sub < 0 in
+    let out = if borrow then pow2 64 + sub else sub in
+    (mk_u64 out, borrow)
+let wrapping_mul_u64 : u64 -> u64 -> u64 = mul_mod
+val saturating_mul_u64 : u64 -> u64 -> u64
+let overflowing_mul_u64 : u64 -> u64 -> u64 & bool = mul_overflow
+let rem_euclid_u64 (x: u64) (y: u64 {v y <> 0}): u64 = x %! y
+val pow_u64 : u64 -> u32 -> u64
+val count_ones_u64 : u64 -> r:u32{v r <= 64}
+
+let wrapping_add_u128 : u128 -> u128 -> u128 = add_mod
+let saturating_add_u128 : u128 -> u128 -> u128 = add_sat
+val overflowing_add_u128 : u128 -> u128 -> u128 & bool
+let wrapping_sub_u128 : u128 -> u128 -> u128 = sub_mod
+let saturating_sub_u128 : u128 -> u128 -> u128 = sub_sat
+let overflowing_sub_u128 (x y: u128): u128 & bool
+  = let sub = v x - v y in
+    let borrow = sub < 0 in
+    let out = if borrow then pow2 128 + sub else sub in
+    (mk_u128 out, borrow)
+let wrapping_mul_u128 : u128 -> u128 -> u128 = mul_mod
+val saturating_mul_u128 : u128 -> u128 -> u128
+let overflowing_mul_u128 : u128 -> u128 -> u128 & bool = mul_overflow
+let rem_euclid_u128 (x: u128) (y: u128 {v y <> 0}): u128 = x %! y
+val pow_u128 : u128 -> u32 -> u128
+val count_ones_u128 : u128 -> r:u32{v r <= 128}
+
+let wrapping_add_usize : usize -> usize -> usize = add_mod
+let saturating_add_usize : usize -> usize -> usize = add_sat
+val overflowing_add_usize : usize -> usize -> usize & bool
+let wrapping_sub_usize : usize -> usize -> usize = sub_mod
+let saturating_sub_usize : usize -> usize -> usize = sub_sat
+let overflowing_sub_usize (x y: usize): usize & bool
+  = let sub = v x - v y in
+    let borrow = sub < 0 in
+    let out = if borrow then pow2 size + sub else sub in
+    (mk_usize out, borrow)
+let wrapping_mul_usize : usize -> usize -> usize = mul_mod
+val saturating_mul_usize : usize -> usize -> usize
+let overflowing_mul_usize : usize -> usize -> usize & bool = mul_overflow
+let rem_euclid_usize (x: usize) (y: usize {v y <> 0}): usize = x %! y
+val pow_usize : usize -> u32 -> usize
+val count_ones_usize : usize -> r:u32{v r <= SIZE_BITS}
+
+let wrapping_add_i8 : i8 -> i8 -> i8 = add_mod
+let saturating_add_i8 : i8 -> i8 -> i8 = add_sat
+val overflowing_add_i8 : i8 -> i8 -> i8 & bool
+let wrapping_sub_i8 : i8 -> i8 -> i8 = sub_mod
+let saturating_sub_i8 : i8 -> i8 -> i8 = sub_sat
+let overflowing_sub_i8 (x y: i8): i8 & bool
+  = let sub = v x - v y in
+    let borrow = sub < 0 in
+    let out = if borrow then pow2 8 + sub else sub in
+    (mk_i8 out, borrow)
+let wrapping_mul_i8 : i8 -> i8 -> i8 = mul_mod
+val saturating_mul_i8 : i8 -> i8 -> i8
+let overflowing_mul_i8 : i8 -> i8 -> i8 & bool = mul_overflow
+let rem_euclid_i8 (x: i8) (y: i8 {v y <> 0}): i8 = x %! y
+val pow_i8 : i8 -> u32 -> i8
+val count_ones_i8 : i8 -> r:u32{v r <= 8}
+
+let wrapping_add_i16 : i16 -> i16 -> i16 = add_mod
+let saturating_add_i16 : i16 -> i16 -> i16 = add_sat
+val overflowing_add_i16 : i16 -> i16 -> i16 & bool
+let wrapping_sub_i16 : i16 -> i16 -> i16 = sub_mod
+let saturating_sub_i16 : i16 -> i16 -> i16 = sub_sat
+let overflowing_sub_i16 (x y: i16): i16 & bool
+  = let sub = v x - v y in
+    let borrow = sub < 0 in
+    let out = if borrow then pow2 16 + sub else sub in
+    (mk_i16 out, borrow)
+let wrapping_mul_i16 : i16 -> i16 -> i16 = mul_mod
+val saturating_mul_i16 : i16 -> i16 -> i16
+let overflowing_mul_i16 : i16 -> i16 -> i16 & bool = mul_overflow
+let rem_euclid_i16 (x: i16) (y: i16 {v y <> 0}): i16 = x %! y
+val pow_i16 : i16 -> u32 -> i16
+val count_ones_i16 : i16 -> r:u32{v r <= 16}
+
+let wrapping_add_i32 : i32 -> i32 -> i32 = add_mod
+let saturating_add_i32 : i32 -> i32 -> i32 = add_sat
+val overflowing_add_i32 : i32 -> i32 -> i32 & bool
+let wrapping_sub_i32 : i32 -> i32 -> i32 = sub_mod
+let saturating_sub_i32 : i32 -> i32 -> i32 = sub_sat
+let overflowing_sub_i32 (x y: i32): i32 & bool
+  = let sub = v x - v y in
+    let borrow = sub < 0 in
+    let out = if borrow then pow2 32 + sub else sub in
+    (mk_i32 out, borrow)
+let wrapping_mul_i32 : i32 -> i32 -> i32 = mul_mod
+val saturating_mul_i32 : i32 -> i32 -> i32
+let overflowing_mul_i32 : i32 -> i32 -> i32 & bool = mul_overflow
+let rem_euclid_i32 (x: i32) (y: i32 {v y <> 0}): i32 = x %! y
+val pow_i32 : i32 -> u32 -> i32
+val count_ones_i32 : i32 -> r:u32{v r <= 32}
+
+let wrapping_add_i64 : i64 -> i64 -> i64 = add_mod
+let saturating_add_i64 : i64 -> i64 -> i64 = add_sat
+val overflowing_add_i64 : i64 -> i64 -> i64 & bool
+let wrapping_sub_i64 : i64 -> i64 -> i64 = sub_mod
+let saturating_sub_i64 : i64 -> i64 -> i64 = sub_sat
+let overflowing_sub_i64 (x y: i64): i64 & bool
+  = let sub = v x - v y in
+    let borrow = sub < 0 in
+    let out = if borrow then pow2 64 + sub else sub in
+    (mk_i64 out, borrow)
+let wrapping_mul_i64 : i64 -> i64 -> i64 = mul_mod
+val saturating_mul_i64 : i64 -> i64 -> i64
+let overflowing_mul_i64 : i64 -> i64 -> i64 & bool = mul_overflow
+let rem_euclid_i64 (x: i64) (y: i64 {v y <> 0}): i64 = x %! y
+val pow_i64 : i64 -> u32 -> i64
+val count_ones_i64 : i64 -> r:u32{v r <= 64}
+
+let wrapping_add_i128 : i128 -> i128 -> i128 = add_mod
+let saturating_add_i128 : i128 -> i128 -> i128 = add_sat
+val overflowing_add_i128 : i128 -> i128 -> i128 & bool
+let wrapping_sub_i128 : i128 -> i128 -> i128 = sub_mod
+let saturating_sub_i128 : i128 -> i128 -> i128 = sub_sat
+let overflowing_sub_i128 (x y: i128): i128 & bool
+  = let sub = v x - v y in
+    let borrow = sub < 0 in
+    let out = if borrow then pow2 128 + sub else sub in
+    (mk_i128 out, borrow)
+let wrapping_mul_i128 : i128 -> i128 -> i128 = mul_mod
+val saturating_mul_i128 : i128 -> i128 -> i128
+let overflowing_mul_i128 : i128 -> i128 -> i128 & bool = mul_overflow
+let rem_euclid_i128 (x: i128) (y: i128 {v y <> 0}): i128 = x %! y
+val pow_i128 : i128 -> u32 -> i128
+val count_ones_i128 : i128 -> r:u32{v r <= 128}
+
+let wrapping_add_isize : isize -> isize -> isize = add_mod
+let saturating_add_isize : isize -> isize -> isize = add_sat
+val overflowing_add_isize : isize -> isize -> isize & bool
+let wrapping_sub_isize : isize -> isize -> isize = sub_mod
+let saturating_sub_isize : isize -> isize -> isize = sub_sat
+let overflowing_sub_isize (x y: isize): isize & bool
+  = let sub = v x - v y in
+    let borrow = sub < 0 in
+    let out = if borrow then pow2 size + sub else sub in
+    (mk_isize out, borrow)
+let wrapping_mul_isize : isize -> isize -> isize = mul_mod
+val saturating_mul_isize : isize -> isize -> isize
+let overflowing_mul_isize : isize -> isize -> isize & bool = mul_overflow
+let rem_euclid_isize (x: isize) (y: isize {v y <> 0}): isize = x %! y
+val pow_isize : isize -> u32 -> isize
+val count_ones_isize : isize -> r:u32{v r <= SIZE_BITS}
